\documentclass{article}
\usepackage[UTF8]{ctex}
\usepackage{amsmath}
\usepackage{amssymb}
\usepackage{esint}
\usepackage{geometry}

\setlength{\parindent}{0em}
\setlength{\parskip}{.5\baselineskip}
%\linespread{1.6}
\pagestyle{empty}
\geometry{a4paper, scale = 0.8}
\begin{document}

\section*{$$\sum_{n=1}^\infty {\frac{1}{1+n^2}}$$}

设$f(x)$周期函数, 周期为$2\pi$, 它在$[-\pi,\pi)$上的表达式为: $f(x) = e^x$. 考虑其傅里叶级数展开:\\
$$
\begin{aligned}
&a_0 = \frac{1}{\pi} \int_{-\pi}^{\pi} {f(x) \mathrm{d}x} =\frac{e^\pi - e^{-\pi}}{\pi} \\
&a_n = \frac{1}{\pi} \int_{-\pi}^{\pi} {f(x) \cos {nx} \mathrm{d}x} = 
\frac{e^\pi - e^{-\pi}}{\pi} \; \frac{(-1)^n}{1+n^2}\\
&b_n = \frac{1}{\pi} \int_{-\pi}^{\pi} {f(x) \sin {nx} \mathrm{d}x}= 
\frac{e^\pi - e^{-\pi}}{\pi} \; \frac{(-1)^{^{n+1}} n }{1+n^2}\\
\end{aligned}
$$
于是:
$$
\begin{aligned}
s(x) &= \frac{a_0}{2} + \sum_{n=1}^\infty  (a_n \cos{nx} + b_n \sin{nx})\\
&= \frac{e^\pi - e^{-\pi}}{2\pi} + \sum_{n=1}^\infty \left(
\frac{e^\pi - e^{-\pi}}{\pi} \; \frac{(-1)^n}{1+n^2} \cos{nx} + 
\frac{e^\pi - e^{-\pi}}{\pi} \; \frac{(-1)^{^{n+1}} n }{1+n^2} \sin{nx}\right)\\
 &= \frac{e^\pi -e^{-\pi}}{\pi} \left[\frac{1}{2} + \sum_{n=1}^\infty \left(\frac{(-1)^n}{1+n^2} \cos{nx} + 
 \frac{(-1)^{^{n+1}}n}{1+n^2} \sin{nx} \right)\right]
\end{aligned}
$$

令$x=\pi$, 可得
$$s(\pi) = \frac{e^\pi -e^{-\pi}}{\pi} \left(\frac{1}{2} + \sum_{n=1}^\infty \frac{1}{1+n^2}\right)$$
同时, 因为$s(x)$是$f(x)$的傅里叶级数展开, $x=\pi$是$f(x)$的间断点, 所以:
$$
\begin{aligned}
s(\pi)&= \frac{1}{2} \left[ \lim_{x \to \pi^{^-}} f(x) + \lim_{x \to \pi^{^+}} f(x) \right] \\
&= \frac{e^\pi + e^{-\pi}}{2}\\
\end{aligned}
$$

所以:
$$
\frac{e^\pi -e^{-\pi}}{\pi} \left(\frac{1}{2} + \sum_{n=1}^\infty \frac{1}{1+n^2}\right) = s(x) = 
\frac{e^\pi + e^{-\pi}}{2}
$$
即:
$$
\sum_{n=1}^\infty \frac{1}{1+n^2} = \frac{e^\pi + e^{-\pi}}{e^\pi - e^{-\pi}} \; \frac{\pi}{2} \; - \; \frac{1}{2}
$$
\end{document}